proofs/compiler/dead_calls_proof.v
@@ -1,6 +1,6 @@
 (* -------------------------------------------------------------------- *)
 From mathcomp Require Import all_ssreflect.
-(* ------- *) Require Import expr compiler_util gen_map dead_calls.
+(* ------- *) Require Import expr compiler_util sem gen_map dead_calls.
 (* ------- *) (* - *) Import PosSet.
 
 Set   Implicit Arguments.
@@ -8,34 +8,184 @@ Unset Strict Implicit.
 Unset Printing Implicit Defensive.
 
 (* -------------------------------------------------------------------- *)
-Lemma i_calls_MkI c ii i :
-  i_calls c (MkI ii i) = i_calls_r c i.
+Fixpoint i_Calls (i : instr) {struct i} : Sp.t :=
+  let: MkI _ i := i in i_Calls_r i
+
+with i_Calls_r (i : instr_r) {struct i} : Sp.t :=
+  let c_Calls (cmd : cmd) :=
+    foldr Sp.union Sp.empty [seq i_Calls c | c <- cmd]
+  in
+
+  match i with
+  | Cassgn _  _  _    => Sp.empty
+  | Copn   _  _  _    => Sp.empty
+  | Cif    _  c1 c2   => Sp.union (c_Calls c1) (c_Calls c2)
+  | Cfor   _  _  c1   => c_Calls c1
+  | Cwhile c1 _  c2   => Sp.union (c_Calls c1) (c_Calls c2)
+  | Ccall  _  _  f  _ => Sp.singleton f
+  end.
+
+Definition c_Calls (cmd : cmd) :=
+  foldr Sp.union Sp.empty [seq i_Calls c | c <- cmd].
+
+(* -------------------------------------------------------------------- *)
+Lemma i_Calls_MkI ii i :
+  i_Calls (MkI ii i) = i_Calls_r i.
 Proof. by []. Qed.
 
-Lemma i_calls_asgn c lv tg e :
-  i_calls_r c (Cassgn lv tg e) = c.
+Lemma i_Calls_asgn lv tg e :
+  i_Calls_r (Cassgn lv tg e) = Sp.empty.
 Proof. by []. Qed.
 
-Lemma i_calls_opn c lv op es :
-  i_calls_r c (Copn lv op es) = c.
+Lemma i_Calls_opn lv op es :
+  i_Calls_r (Copn lv op es) = Sp.empty.
 Proof. by []. Qed.
 
-Lemma i_calls_if c e c1 c2 :
-  i_calls_r c (Cif e c1 c2) = c_calls (c_calls c c1) c2.
+Lemma i_Calls_if e c1 c2 :
+  i_Calls_r (Cif e c1 c2) = Sp.union (c_Calls c1) (c_Calls c2).
 Proof. by []. Qed.
 
-Lemma i_calls_for c v rg c1 :
-  i_calls_r c (Cfor v rg c1) = c_calls c c1.
+Lemma i_Calls_for v rg c1 :
+  i_Calls_r (Cfor v rg c1) = c_Calls c1.
 Proof. by []. Qed.
 
-Lemma i_calls_while c c1 e c2 :
-  i_calls_r c (Cwhile c1 e c2) = c_calls (c_calls c c1) c2.
+Lemma i_Calls_while c1 e c2 :
+  i_Calls_r (Cwhile c1 e c2) = Sp.union (c_Calls c1) (c_Calls c2).
 Proof. by []. Qed.
 
-Lemma i_calls_call c ii lv f es :
-  i_calls_r c (Ccall ii lv f es) = Sp.add f c.
+Lemma i_Calls_call ii lv f es :
+  i_Calls_r (Ccall ii lv f es) = Sp.singleton f.
 Proof. by []. Qed.
 
-Hint Rewrite i_calls_MkI  i_calls_asgn i_calls_opn   : calls.
-Hint Rewrite i_calls_if   i_calls_for  i_calls_while : calls.
-Hint Rewrite i_calls_call : calls.
+Lemma c_Calls_nil : c_Calls [::] = Sp.empty.
+Proof. by []. Qed.
+
+Lemma c_Calls_cons i c : c_Calls (i :: c) = Sp.union (i_Calls i) (c_Calls c).
+Proof. by []. Qed.
+
+Hint Rewrite i_Calls_MkI  i_Calls_asgn i_Calls_opn   : calls.
+Hint Rewrite i_Calls_if   i_Calls_for  i_Calls_while : calls.
+Hint Rewrite i_Calls_call c_Calls_nil  c_Calls_cons  : calls.
+
+Definition CallsE :=
+  (i_Calls_MkI , i_Calls_asgn, i_Calls_opn  ,
+   i_Calls_if  , i_Calls_for , i_Calls_while,
+   i_Calls_call, c_Calls_nil , c_Calls_cons ).
+
+(* -------------------------------------------------------------------- *)
+Lemma i_callsE c i : i_calls c i = Sp.union c (i_Calls i).
+Proof. Admitted.
+
+Lemma c_callsE c i : c_calls c i = Sp.union c (c_Calls i).
+Proof. Admitted.
+
+(* -------------------------------------------------------------------- *)
+Lemma dead_calls_subseq c p : subseq (dead_calls c p) p.
+Proof.
+elim: p c => [|[f fd] p ih] c //=; case: ifPn => _; last first.
++ case E: (dead_calls _ _) => [//|[f' fd'] p'].
+  case: ifPn => _; last by rewrite -E. have := ih c.
+  by rewrite E => /(subseq_trans _); apply; apply/subseq_cons.
+by rewrite eqxx c_callsE; apply: ih.
+Qed.
+
+(* -------------------------------------------------------------------- *)
+Section PgCompat.
+Variables (c : Sp.t) (p p' : prog).
+
+Definition pg_compat_cmd :=
+  forall m cmd m', sem p m cmd m' -> sem p' m cmd m'.
+
+Definition pg_compat_Instr :=
+  forall m i m', sem_I p m i m' -> sem_I p' m i m'.
+
+Definition pg_compat_instr :=
+  forall m i m', sem_i p m i m' -> sem_i p' m i m'.
+
+Definition pg_compat_for :=
+  forall v rg m cmd m',
+    sem_for p v rg m cmd m' -> sem_for p' v rg m cmd m'.
+
+Definition pg_compat_call :=
+  forall m f args m' res, Sp.In f c ->
+    sem_call p  m f args m' res ->
+    sem_call p' m f args m' res.
+End PgCompat.
+
+(* -------------------------------------------------------------------- *)
+Lemma pg_compat_sub c1 c2 p p' : Sp.Subset c2 c1 ->
+     pg_compat_call c1 p p'
+  -> pg_compat_call c2 p p'.
+Proof.
+by move=> lt h m f args m' res f_in_c2 /h; apply; SpD.fsetdec.
+Qed.
+
+Lemma pg_compat_cmd_consl i c p p' :
+     pg_compat_call (c_Calls (i :: c)) p p'
+  -> pg_compat_call (i_Calls i) p p'.
+Proof.
+by apply: pg_compat_sub; rewrite CallsE; SpD.fsetdec.
+Qed.
+
+Lemma pg_compat_cmd_consr i c p p' :
+     pg_compat_call (c_Calls (i :: c)) p p'
+  -> pg_compat_call (c_Calls c) p p'.
+Proof.
+by apply: pg_compat_sub; rewrite CallsE; SpD.fsetdec.
+Qed.
+
+Lemma pg_compat_while_pre c e c' p p' :
+     pg_compat_call (i_Calls_r (Cwhile c e c')) p p'
+  -> pg_compat_call (c_Calls c) p p'.
+Proof.
+by apply: pg_compat_sub; rewrite CallsE; SpD.fsetdec.
+Qed.
+
+Lemma pg_compat_while_post c e c' p p' :
+     pg_compat_call (i_Calls_r (Cwhile c e c')) p p'
+  -> pg_compat_call (c_Calls c') p p'.
+Proof.
+by apply: pg_compat_sub; rewrite CallsE; SpD.fsetdec.
+Qed.
+
+Lemma pg_compat_for_body v rg c p p' :
+     pg_compat_call (i_Calls_r (Cfor v rg c)) p p'
+  -> pg_compat_call (c_Calls c) p p'.
+Proof.
+by apply: pg_compat_sub; rewrite CallsE; SpD.fsetdec.
+Qed.
+
+(* -------------------------------------------------------------------- *)
+Local Hint Resolve pg_compat_cmd_consl pg_compat_cmd_consr.
+Local Hint Resolve pg_compat_while_pre pg_compat_while_post.
+Local Hint Resolve pg_compat_for_body.
+Local Hint Constructors sem sem_I sem_i sem_for sem_call.
+
+(* -------------------------------------------------------------------- *)
+Lemma ok p m f args m' res fd p' :
+     pg_compat_call (c_Calls fd.(f_body)) p p'
+  -> sem_call ((f, fd) :: p ) m f args m' res
+  -> sem_call ((f, fd) :: p') m f args m' res.
+Proof.
+pose Pc m c m' :=
+     pg_compat_call (c_Calls c) p p'
+  -> sem p m c m' -> sem p' m c m'.
+pose PI m i m' :=
+     pg_compat_call (i_Calls i) p p'
+  -> sem_I p m i m' -> sem_I p' m i m'.
+pose Pi m i m' :=
+     pg_compat_call (i_Calls_r i) p p'
+  -> sem_i p m i m' -> sem_i p' m i m'.
+pose Pf v rg m c m' :=
+     pg_compat_call (c_Calls c) p p'
+  -> sem_for p v rg m c m' -> sem_for p' v rg m c m'.
+pose PC m f args m' res :=
+     pg_compat_call (c_Calls fd.(f_body)) p p'
+  -> sem_call ((f, fd) :: p ) m f args m' res
+  -> sem_call ((f, fd) :: p') m f args m' res.
+apply: (@sem_call_Ind p Pc Pi PI Pf PC);
+  rewrite {}/Pc {}/Pi {}/PI {}/Pf {}/PC; try by eauto 7.
++ admit.
++ admit.
++ admit.
+Admitted.
